AwsCryptographicMaterialProviders/dafny/AwsCryptographyKeyStoreAdmin/src/InitializeMutation.dfy
@@ -385,7 +385,7 @@ module {:options "/functionSyntax:4" } InternalInitializeMutation {
     returns (res: Result<KeyStoreTypes.EncryptedHierarchicalKey, Types.Error>)
     requires KmsArn.ValidKmsArn?(mutationToApply.Terminal.kmsArn)
     requires KMSKeystoreOperations.AttemptKmsOperation?(
-               KeyStoreTypes.kmsKeyArn(mutationToApply.Terminal.kmsArn), decryptOnlyEncryptionContext
+               KeyStoreTypes.kmsKeyArn(mutationToApply.Terminal.kmsArn), decryptOnlyEncryptionContext[Structure.KMS_FIELD]
              )
     requires keyManagerStrategy.ValidState()
     requires keyManagerStrategy.SupportHV1()
@@ -393,7 +393,7 @@ module {:options "/functionSyntax:4" } InternalInitializeMutation {
     ensures keyManagerStrategy.ValidState()
     ensures res.Success? ==>
               && Structure.BranchKeyContext?(res.value.EncryptionContext)
-              && Structure.EncryptedHierarchicalKey?(res.value)
+              && Structure.EncryptedHierarchicalKeyFromStorage?(res.value)
               && res.value.KmsArn == KMSKeystoreOperations.GetKeyId(KeyStoreTypes.kmsKeyArn(mutationToApply.Terminal.kmsArn))
               && Structure.BRANCH_KEY_TYPE_PREFIX < res.value.EncryptionContext[Structure.TYPE_FIELD]
               && Structure.BRANCH_KEY_ACTIVE_VERSION_FIELD !in decryptOnlyEncryptionContext
@@ -568,7 +568,7 @@ module {:options "/functionSyntax:4" } InternalInitializeMutation {
       && 0 < |timestamp|
       && 0 < |input.Identifier|
       && activeItem.KmsArn == mutationToApply.Original.kmsArn
-      && Structure.EncryptedHierarchicalKey?(activeItem)
+      && Structure.EncryptedHierarchicalKeyFromStorage?(activeItem)
       && input.keyManagerStrategy.SupportHV1()
     }
 
